src/datalog/ForwardingNode.v
@@ -5,62 +5,6 @@ From coqutil Require Import Map.Interface Map.Properties.
 From coqutil Require Import Eqb Semantics.OmniSmallstepCombinators Tactics Tactics.fwd.
 Import ListNotations.
 
-Variant source :=
-  | node_source (_ : node_id)
-  | input_source.
-
-#[export] Instance source_eqb : Eqb source :=
-  fun s1 s2 =>
-    match s1, s2 with
-    | node_source n1, node_source n2 => eqb n1 n2
-    | input_source, input_source => true
-    | _, _ => false
-    end.
-
-#[export] Instance source_eqb_ok : Eqb_ok source_eqb.
-Proof.
-  intros a b. destruct a, b; cbn; try congruence.
-  destr (eqb n n0); congruence.
-Qed.
-
-Variant destn :=
-  | node_destn (_ : node_id)
-  | output_destn.
-
-#[export] Instance destn_eqb : Eqb destn :=
-  fun d1 d2 =>
-    match d1, d2 with
-    | node_destn n1, node_destn n2 => eqb n1 n2
-    | output_destn, output_destn => true
-    | _, _ => false
-    end.
-
-#[export] Instance destn_eqb_ok : Eqb_ok destn_eqb.
-Proof.
-  intros a b. destruct a, b; cbn; try congruence.
-  destr (eqb n n0); congruence.
-Qed.
-
-Variant location :=
-  | node_loc (_ : node_id)
-  | input_loc
-  | output_loc.
-
-#[export] Instance location_eqb : Eqb location :=
-  fun l1 l2 =>
-    match l1, l2 with
-    | node_loc n1, node_loc n2 => eqb n1 n2
-    | input_loc, input_loc => true
-    | output_loc, output_loc => true
-    | _, _ => false
-    end.
-
-#[export] Instance location_eqb_ok : Eqb_ok location_eqb.
-Proof.
-  intros a b. destruct a, b; cbn; try congruence.
-  destr (eqb n n0); congruence.
-Qed.
-
 Definition loc_of_source (s : source) : location :=
   match s with
   | node_source n => node_loc n
@@ -187,16 +131,11 @@ Section __.
 
   Definition ngraph_step :=
     graph_step
-      (fun src dst m => inb (node_destn dst) (nforward (node_source src) (dfact_rel m)))
-      (fun dst m => inb (node_destn dst) (nforward input_source (dfact_rel m)))
-      (fun n f => inb output_destn (nforward (node_source n) (dfact_rel f)))
+      (fun s d m => inb d (nforward s (dfact_rel m)))
       (fun n => node_step (prog_at n)).
 
-  Definition fforward (src : node_id) (mn : rel * source) : list destn :=
-    get_or_default (get_or_default fts (node_source src)) mn.
-
-  Definition finput_locs R : list destn :=
-    get_or_default (get_or_default fts input_source) (R, input_source).
+  Definition fforward (s : source) (mn : rel * source) : list destn :=
+    get_or_default (get_or_default fts s) mn.
 
   Definition corresp (e : IO_event) (e' : fIO_event) : Prop :=
     match e with
@@ -212,9 +151,7 @@ Section __.
     exists e',
       corresp e e' /\
         graph_step
-          (fun src dst '(f, orig) => inb (node_destn dst) (fforward src (dfact_rel f, orig)))
-          finput_at
-          foutput_visible
+          (fun s d '(f, orig) => inb d (fforward s (dfact_rel f, orig)))
           (fun n => fnode_step node_step (fprog_at n) n)
           g1 e' g2.
 
